WIP

PatchTheorems.lean
@@ -1,78 +1,111 @@
+prelude
+import Init.Prelude
+import Init.Notation
+import Init.Core
+
+namespace L4L
+
+noncomputable def cast {α β : Sort u} (h : Eq α β) (a : α) : β :=
+  h.rec a
+
 axiom prfIrrelHEq (P Q : Prop) (heq : P = Q) (p : Q) (q : P) : HEq p q
 
 theorem appArgHEq {A : Sort u} {U : A → Sort v}
   (f : (a : A) → U a)
   {a b : A} (hab : HEq a b)
-  : HEq (f a) (f b) := by
-  subst hab
-  rfl
-
-theorem appArgHEq' {A B : Sort u} (hBA : B = A) {U : A → Sort v}
-  (f : (a : A) → U a)
-  {a : A} {b : B} (hab : HEq a b)
-  : HEq (f a) (f (cast hBA b)) := by
-  subst hBA
-  subst hab
-  rfl
-
-structure S : Type where
-u : Nat
-
-theorem projHEqStruct (a b : S) (hab : a = b) : a.u = b.u := by
-  subst hab
-  rfl
-
-inductive K : Nat → Prop where
-  | mk : K 1
-#check K.rec
-
-theorem KRedKLike (h : K 1) 
-  : (@K.rec (fun _ _ => Nat) 10 1 h) = 10 := rfl
+  : HEq (f a) (f b) :=
+  @Eq.ndrec A a (fun {b : A} => @HEq (U a) (f a) (U b) (f b)) (@HEq.rfl (U a) (f a)) b (@eq_of_heq A a b hab)
 
 theorem appHEq {A B : Sort u} {U : A → Sort v} {V : B → Sort v}
   (hAB : A = B) (hUV : (a : A) → (b : B) → HEq a b → HEq (U a) (V b))
   {f : (a : A) → U a} {g : (b : B) → V b} {a : A} {b : B}
   (hfg : HEq f g) (hab : HEq a b)
-  : HEq (f a) (g b) := by
-  subst hAB
-  have : U = V := by
-    apply funext
-    intro x
-    exact eq_of_heq (hUV x x HEq.rfl)
-  subst this
-  subst hab
-  subst hfg
-  rfl
+  : HEq (f a) (g b) :=
+  @Eq.ndrec (Sort u) A
+    (fun {B : Sort u} =>
+      ∀ {V : B → Sort v},
+        (∀ (a : A) (b : B), @HEq A a B b → @HEq (Sort v) (U a) (Sort v) (V b)) →
+          ∀ {g : (b : B) → V b} {b : B},
+            @HEq ((a : A) → U a) f ((b : B) → V b) g → @HEq A a B b → @HEq (U a) (f a) (V b) (g b))
+    (fun {V : A → Sort v} (hUV : ∀ (a b : A), @HEq A a A b → @HEq (Sort v) (U a) (Sort v) (V b)) {g : (b : A) → V b}
+        {b : A} (hfg : @HEq ((a : A) → U a) f ((b : A) → V b) g) (hab : @HEq A a A b) =>
+      @letFun (@Eq (A → Sort v) U V) (fun (_ : @Eq (A → Sort v) U V) => @HEq (U a) (f a) (V b) (g b))
+        (@funext A (fun (_ : A) => Sort v) U V fun (x : A) => @eq_of_heq (Sort v) (U x) (V x) (hUV x x (@HEq.rfl A x)))
+        fun (this : @Eq (A → Sort v) U V) =>
+        @Eq.ndrec (A → Sort v) U
+          (fun {V : A → Sort v} =>
+            (∀ (a b : A), @HEq A a A b → @HEq (Sort v) (U a) (Sort v) (V b)) →
+              ∀ {g : (b : A) → V b}, @HEq ((a : A) → U a) f ((b : A) → V b) g → @HEq (U a) (f a) (V b) (g b))
+          (fun (_ : ∀ (a b : A), @HEq A a A b → @HEq (Sort v) (U a) (Sort v) (U b)) {g : (b : A) → U b}
+              (hfg : @HEq ((a : A) → U a) f ((b : A) → U b) g) =>
+            @Eq.ndrec A a (fun {b : A} => @HEq (U a) (f a) (U b) (g b))
+              (@Eq.ndrec ((a : A) → U a) f (fun {g : (b : A) → U b} => @HEq (U a) (f a) (U a) (g a))
+                (@HEq.rfl (U a) (f a)) g (@eq_of_heq ((a : A) → U a) f g hfg))
+              b (@eq_of_heq A a b hab))
+          V this hUV g hfg)
+    B hAB V hUV g b hfg hab
 
-theorem appHEqBinNatFn {T : Type}
-  {f : Nat → Nat → T} {a1 a2 : Nat} {b1 b2 : Nat}
+theorem appHEqBinNatFn {N : Type} {T : Type}
+  {f : N → N → T} {a1 a2 : N} {b1 b2 : N}
   (ha : HEq a1 a2)
   (hb : HEq b1 b2)
-  : HEq (f a1 b1) (f a2 b2) := by
-  subst ha
-  subst hb
-  rfl
+  : HEq (f a1 b1) (f a2 b2) :=
+  @Eq.ndrec N a1 (fun {a2 : N} => @HEq T (f a1 b1) T (f a2 b2))
+    (@Eq.ndrec N b1 (fun {b2 : N} => @HEq T (f a1 b1) T (f a1 b2)) (@HEq.rfl T (f a1 b1)) b2
+      (@eq_of_heq N b1 b2 hb))
+    a2 (@eq_of_heq N a1 a2 ha)
 
 theorem lambdaHEq {A B : Sort u} {U : A → Sort v} {V : B → Sort v}
   (f : (a : A) → U a) (g : (b : B) → V b)
   (hAB : A = B) (hfg : (a : A) → (b : B) → HEq a b → HEq (f a) (g b))
-  : HEq (fun a => f a) (fun b => g b) := by
-  subst hAB
-  have hUV : U = V := by
-    apply funext
-    intro x
-    exact type_eq_of_heq (hfg x x HEq.rfl)
-  subst hUV
-  have : f = g := funext fun a => eq_of_heq $ hfg a a HEq.rfl
-  exact heq_of_eq this
+  : HEq (fun a => f a) (fun b => g b) :=
+  @Eq.ndrec (Sort u) A
+    (fun {B : Sort u} =>
+      ∀ {V : B → Sort v} (g : (b : B) → V b),
+        (∀ (a : A) (b : B), @HEq A a B b → @HEq (U a) (f a) (V b) (g b)) →
+          @HEq ((a : A) → U a) (fun (a : A) => f a) ((b : B) → V b) fun (b : B) => g b)
+    (fun {V : A → Sort v} (g : (b : A) → V b) (hfg : ∀ (a b : A), @HEq A a A b → @HEq (U a) (f a) (V b) (g b)) =>
+      @letFun (@Eq (A → Sort v) U V)
+        (fun (_ : @Eq (A → Sort v) U V) =>
+          @HEq ((a : A) → U a) (fun (a : A) => f a) ((b : A) → V b) fun (b : A) => g b)
+        (@funext A (fun (_ : A) => Sort v) U V fun (x : A) =>
+          @type_eq_of_heq (U x) (V x) (f x) (g x) (hfg x x (@HEq.rfl A x)))
+        fun (hUV : @Eq (A → Sort v) U V) =>
+        @Eq.ndrec (A → Sort v) U
+          (fun {V : A → Sort v} =>
+            ∀ (g : (b : A) → V b),
+              (∀ (a b : A), @HEq A a A b → @HEq (U a) (f a) (V b) (g b)) →
+                @HEq ((a : A) → U a) (fun (a : A) => f a) ((b : A) → V b) fun (b : A) => g b)
+          (fun (g : (b : A) → U b) (hfg : ∀ (a b : A), @HEq A a A b → @HEq (U a) (f a) (U b) (g b)) =>
+            @letFun (@Eq ((a : A) → U a) f g)
+              (fun (_ : @Eq ((a : A) → U a) f g) =>
+                @HEq ((a : A) → U a) (fun (a : A) => f a) ((b : A) → U b) fun (b : A) => g b)
+              (@funext A (fun (x : A) => U x) f g fun (a : A) => @eq_of_heq (U a) (f a) (g a) (hfg a a (@HEq.rfl A a)))
+              fun (this : @Eq ((a : A) → U a) f g) =>
+              @heq_of_eq ((a : A) → U a) (fun (a : A) => f a) (fun (b : A) => g b) this)
+          V hUV g hfg)
+    B hAB V g hfg
 
 theorem forAllHEq {A B : Sort u} {U : A → Sort v} {V : B → Sort v}
   (hAB : A = B) (hUV : (a : A) → (b : B) → HEq a b → HEq (U a) (V b))
-  : ((a : A) → U a) = ((b : B) → V b) := by
-  subst hAB
-  have : U = V := by
-    apply funext
-    intro x
-    exact eq_of_heq $ hUV x x HEq.rfl
-  subst this
-  rfl
+  : ((a : A) → U a) = ((b : B) → V b) :=
+  @Eq.ndrec (Sort u) A
+    (fun {B : Sort u} =>
+      ∀ {V : B → Sort v},
+        (∀ (a : A) (b : B), @HEq A a B b → @HEq (Sort v) (U a) (Sort v) (V b)) →
+          @Eq (Sort (imax u v)) ((a : A) → U a) ((b : B) → V b))
+    (fun {V : A → Sort v} (hUV : ∀ (a b : A), @HEq A a A b → @HEq (Sort v) (U a) (Sort v) (V b)) =>
+      @letFun (@Eq (A → Sort v) U V)
+        (fun (_ : @Eq (A → Sort v) U V) => @Eq (Sort (imax u v)) ((a : A) → U a) ((b : A) → V b))
+        (@funext A (fun (_ : A) => Sort v) U V fun (x : A) => @eq_of_heq (Sort v) (U x) (V x) (hUV x x (@HEq.rfl A x)))
+        fun (this : @Eq (A → Sort v) U V) =>
+        @Eq.ndrec (A → Sort v) U
+          (fun {V : A → Sort v} =>
+            (∀ (a b : A), @HEq A a A b → @HEq (Sort v) (U a) (Sort v) (V b)) →
+              @Eq (Sort (imax u v)) ((a : A) → U a) ((b : A) → V b))
+          (fun (_ : ∀ (a b : A), @HEq A a A b → @HEq (Sort v) (U a) (Sort v) (U b)) =>
+            @Eq.refl (Sort (imax u v)) ((a : A) → U a))
+          V this hUV)
+    B hAB V hUV
+
+end L4L
